lib/list.fst
@@ -29,73 +29,73 @@ let hd = function
   | hd::tl -> hd
   | _ -> failwith "head of empty list"
 
-let tail = function
-  | hd::tl -> tl
-  | _ -> failwith "tail of empty list"
+(* let tail = function *)
+(*   | hd::tl -> tl *)
+(*   | _ -> failwith "tail of empty list" *)
 
-val mem: 'a -> list 'a -> bool //x:'a -> l:list 'a -> b:bool{b==true <==> In x l}
-let rec mem x = function
-  | [] -> false
-  | hd::tl -> if hd = x then true else mem x tl
+(* val mem: 'a -> list 'a -> bool //x:'a -> l:list 'a -> b:bool{b==true <==> In x l} *)
+(* let rec mem x = function *)
+(*   | [] -> false *)
+(*   | hd::tl -> if hd = x then true else mem x tl *)
 
-val map: ('a -> 'b) -> list 'a -> list 'b
-let rec map f x = match x with
-  | [] -> []
-  | a::tl -> f a::map f tl
+(* val map: ('a -> 'b) -> list 'a -> list 'b *)
+(* let rec map f x = match x with *)
+(*   | [] -> [] *)
+(*   | a::tl -> f a::map f tl *)
 
-val fold_left: ('a -> 'b -> 'a) -> 'a -> list 'b -> 'a
-let rec fold_left f x y = match y with
-  | [] -> x
-  | hd::tl -> fold_left f (f x hd) tl
+(* val fold_left: ('a -> 'b -> 'a) -> 'a -> list 'b -> 'a *)
+(* let rec fold_left f x y = match y with *)
+(*   | [] -> x *)
+(*   | hd::tl -> fold_left f (f x hd) tl *)
 
-val fold_right: ('a -> 'b -> 'b) -> list 'a -> 'b -> 'b
-let rec fold_right f l x = match l with
-  | [] -> x
-  | hd::tl -> fold_right f tl (f hd x)
+(* val fold_right: ('a -> 'b -> 'b) -> list 'a -> 'b -> 'b *)
+(* let rec fold_right f l x = match l with *)
+(*   | [] -> x *)
+(*   | hd::tl -> fold_right f tl (f hd x) *)
 
-val iter: ('a -> unit) -> list 'a -> unit
-let rec iter f x = match x with
-  | [] -> ()
-  | a::tl -> let _ = f a in iter f tl
+(* val iter: ('a -> unit) -> list 'a -> unit *)
+(* let rec iter f x = match x with *)
+(*   | [] -> () *)
+(*   | a::tl -> let _ = f a in iter f tl *)
                                   
-val assoc: 'a -> list ('a*'b) -> option 'b
-let rec assoc a x = match x with
-  | [] -> None
-  | (a', b)::tl -> if a=a' then Some b else assoc a tl
+(* val assoc: 'a -> list ('a*'b) -> option 'b *)
+(* let rec assoc a x = match x with *)
+(*   | [] -> None *)
+(*   | (a', b)::tl -> if a=a' then Some b else assoc a tl *)
 
-val append: list 'a -> list 'a -> list 'a //x:list 'a -> y:list 'a -> z:list 'a { forall (a:'a). In a z <==> In a x \/ In a y }
-let rec append x y = match x with
-  | [] -> y
-  | a::tl -> a::append tl y
+(* val append: list 'a -> list 'a -> list 'a //x:list 'a -> y:list 'a -> z:list 'a { forall (a:'a). In a z <==> In a x \/ In a y } *)
+(* let rec append x y = match x with *)
+(*   | [] -> y *)
+(*   | a::tl -> a::append tl y *)
 
-val concatMap: ('a -> list 'b) -> list 'a -> list 'b
-let rec concatMap f = function
-  | [] -> []
-  | a::tl ->
-    let fa = f a in
-    let ftl = concatMap f tl in
-    append fa ftl
+(* val concatMap: ('a -> list 'b) -> list 'a -> list 'b *)
+(* let rec concatMap f = function *)
+(*   | [] -> [] *)
+(*   | a::tl -> *)
+(*     let fa = f a in *)
+(*     let ftl = concatMap f tl in *)
+(*     append fa ftl *)
 
-assume val forall2: ('a -> 'b -> bool) -> list 'a -> list 'b -> bool
-assume val mapi: (int -> 'a -> 'b) -> list 'a -> list 'b
-assume val map2: ('a -> 'b -> 'c) -> list 'a -> list 'b -> list 'c
-assume val split: list ('a * 'b) -> PURE.Tot (list 'a * list 'b)
-assume val unzip: list ('a * 'b) -> PURE.Tot (list 'a * list 'b)
-assume val unzip3: list ('a * 'b * 'c) -> PURE.Tot (list 'a * list 'b * list 'c)
-assume val zip: list 'a -> list 'b -> PURE.Tot (list ('a * 'b))
-assume val zip3: list 'a -> list 'b -> list 'c -> PURE.Tot (list ('a * 'b * 'c))
-assume val map3: ('a -> 'b -> 'c -> 'd) -> list 'a -> list 'b -> list 'c -> list 'd
-assume val rev: list 'a -> PURE.Tot (list 'a)
-assume val collect: ('a -> list 'b) -> list 'a -> list 'b
-assume val tl: list 'a -> list 'a
-assume val length: list 'a -> PURE.Tot int
-assume val tryFind: ('a -> bool) -> list 'a -> option 'b
-assume val concat: list (list 'a) -> PURE.Tot (list 'a)
-assume val sortWith: ('a -> 'a -> int) -> list 'a -> list 'a
-assume val choose: ('a -> option 'b) -> list 'a -> list 'b
-assume val flatten: list (list 'a) -> PURE.Tot (list 'a)
-assume val filter: ('a -> bool) -> list 'a -> list 'a
-assume val partition: ('a -> bool) -> list 'a -> (list 'a * list 'a)
-assume val contains: 'a -> list 'a -> PURE.Tot bool
-assume val fold_left2: ('s -> 'a -> 'b -> 's) -> 's -> list 'a -> list 'b -> 's
+(* assume val forall2: ('a -> 'b -> bool) -> list 'a -> list 'b -> bool *)
+(* assume val mapi: (int -> 'a -> 'b) -> list 'a -> list 'b *)
+(* assume val map2: ('a -> 'b -> 'c) -> list 'a -> list 'b -> list 'c *)
+(* assume val split: list ('a * 'b) -> PURE.Tot (list 'a * list 'b) *)
+(* assume val unzip: list ('a * 'b) -> PURE.Tot (list 'a * list 'b) *)
+(* assume val unzip3: list ('a * 'b * 'c) -> PURE.Tot (list 'a * list 'b * list 'c) *)
+(* assume val zip: list 'a -> list 'b -> PURE.Tot (list ('a * 'b)) *)
+(* assume val zip3: list 'a -> list 'b -> list 'c -> PURE.Tot (list ('a * 'b * 'c)) *)
+(* assume val map3: ('a -> 'b -> 'c -> 'd) -> list 'a -> list 'b -> list 'c -> list 'd *)
+(* assume val rev: list 'a -> PURE.Tot (list 'a) *)
+(* assume val collect: ('a -> list 'b) -> list 'a -> list 'b *)
+(* assume val tl: list 'a -> list 'a *)
+(* assume val length: list 'a -> PURE.Tot int *)
+(* assume val tryFind: ('a -> bool) -> list 'a -> option 'b *)
+(* assume val concat: list (list 'a) -> PURE.Tot (list 'a) *)
+(* assume val sortWith: ('a -> 'a -> int) -> list 'a -> list 'a *)
+(* assume val choose: ('a -> option 'b) -> list 'a -> list 'b *)
+(* assume val flatten: list (list 'a) -> PURE.Tot (list 'a) *)
+(* assume val filter: ('a -> bool) -> list 'a -> list 'a *)
+(* assume val partition: ('a -> bool) -> list 'a -> (list 'a * list 'a) *)
+(* assume val contains: 'a -> list 'a -> PURE.Tot bool *)
+(* assume val fold_left2: ('s -> 'a -> 'b -> 's) -> 's -> list 'a -> list 'b -> 's *)
 
